Cleanups

proof/Simple/EsJudge.v
@@ -3,7 +3,7 @@ Require Export Exp.
 Require Export SubstValueValue.
 
 
-(* Small Step Evaluation ********************************************)
+(* Single Small Step Evaluation ************************************)
 Inductive STEP : exp -> exp -> Prop :=
  | ESLamApp
    : forall t11 x12 v2
@@ -25,7 +25,39 @@ Inductive STEP : exp -> exp -> Prop :=
 Hint Constructors STEP.
 
 
+(* Multi-step evaluation *******************************************)
+Inductive STEPS : nat -> exp -> exp -> Prop :=
+ | ESDone
+   :  forall x1
+   ,  STEPS 0 x1 x1
+
+ | ESStep
+   :  forall x1 x2
+   ,  STEP  x1 x2
+   -> STEPS 1 x1 x2
+
+ | ESLink
+   :  forall n1 n2 x1 x2 x3
+   ,  STEPS n1 x1 x2 -> STEPS n2 x2 x3
+   -> STEPS (n1 + n2) x1 x3.
+
+Hint Constructors STEPS.
 
 
+Lemma steps_app1
+ :  forall n x1 x1' x2
+ ,  STEPS n x1 x1'
+ -> STEPS n (XApp x1 x2) (XApp x1' x2).
+Proof.
+ intros. induction H; eauto.
+Qed.
 
 
+Lemma steps_app2
+ :  forall n v1 x2 x2'
+ ,  value v1 
+ -> STEPS n x2 x2'
+ -> STEPS n (XApp v1 x2) (XApp v1 x2').
+Proof.
+ intros. induction H0; eauto.
+Qed.
