proof/Simple/EvJudge.v
@@ -6,40 +6,6 @@ Require Export EsJudge.
 Require Export Exp.
 
 
-(* Multi-step evaluation ********************************************)
-Inductive STEPS : nat -> exp -> exp -> Prop :=
- | ESDone
-   :  forall x1
-   ,  STEPS 0 x1 x1
-
- | ESStep
-   :  forall x1 x2
-   ,  STEP  x1 x2
-   -> STEPS 1 x1 x2
-
- | ESLink
-   :  forall n1 n2 x1 x2 x3
-   ,  STEPS n1 x1 x2 -> STEPS n2 x2 x3
-   -> STEPS (n1 + n2) x1 x3.
-
-Hint Constructors STEPS.
-
-
-(* When we multi-step evaluate some expression,
-   then the result has the same type as the original.
- *)  
-Lemma preservation_steps
- :  forall n x1 t1 x2
- ,  TYPE Empty x1 t1
- -> STEPS n    x1 x2
- -> TYPE Empty x2 t1.
-Proof.
- intros. 
- induction H0; eauto.
-  eapply preservation; eauto.
-Qed.
-
-
 (* Big Step Evaluation **********************************************)
 Inductive EVAL : exp -> exp -> Prop :=
  | EvValue
@@ -49,42 +15,19 @@ Inductive EVAL : exp -> exp -> Prop :=
 
  | EvLamApp
    :  forall x1 t11 x12 x2 v2 v3
-   ,  value v2
-   -> value v3
-   -> EVAL x1 (XLam t11 x12)
-   -> EVAL x2 v2
-   -> EVAL (subst v2 x12) v3
+   ,                              value v2               -> value v3
+   -> EVAL x1 (XLam t11 x12) -> EVAL x2 v2 -> EVAL (subst v2 x12) v3
    -> EVAL (XApp x1 x2) v3.
 
 Hint Constructors EVAL.
 
 
-Lemma steps_app1
- :  forall n x1 x1' x2
- ,  STEPS n x1 x1'
- -> STEPS n (XApp x1 x2) (XApp x1' x2).
-Proof.
- intros. 
- induction H; eauto.
-Qed.
-
-
-Lemma steps_app2
- :  forall n v1 x2 x2'
- ,  value v1 
- -> STEPS n x2 x2'
- -> STEPS n (XApp v1 x2) (XApp v1 x2').
-Proof.
- intros.
- induction H0; eauto.
-Qed.
-
-
+(* Big to Small steps ***********************************************)
 Lemma eval_to_steps
- :  forall x1 t1 v2
+ :  forall x1 t1 x2
  ,  TYPE Empty x1 t1
- -> EVAL x1 v2
- -> (exists n,  STEPS n x1 v2).
+ -> EVAL x1 x2
+ -> (exists n,  STEPS n x1 x2).
 Proof.
  intros x1 t1 v2 HT HE. gen t1.
  induction HE.
